Demostracion de la aproximacion

Algoritmos Aproximados/Envasado.dfy/Algoritmo2AproximadoAux.dfy
@@ -1,20 +1,23 @@
-include "../../Especificaciones/Envasado/Envasado.dfy"
+include "../../Especificaciones/Envasado/EnvasadoProperties.dfy"
 include "EnvasadoKAproximado.dfy"
 
 //All bins are more than half full
 //Used locally
-predicate allMoreThanHalfFull(E: nat, I: multiset<multiset<nat>>)
+ghost predicate allMoreThanHalfFull(E: nat, I: multiset<multiset<nat>>)
 {
-    (forall M: multiset<nat> | M in I :: FSumNat(M) * 2 > E)
+    (forall M: multiset<nat> | M in I :: GSumNat(M) * 2 > E)
 }
+
 
 //Only one bin in I is less than half full
 //Used locally
-predicate oneLessThanHalfFull(E: nat, I: multiset<multiset<nat>>)
+ghost predicate oneLessThanHalfFull(E: nat, I: multiset<multiset<nat>>)
 {
-    (exists M: multiset<nat> :: M in I && FSumNat(M) * 2 <= E && (forall M': multiset<nat> | M' in I && FSumNat(M') * 2 <= E :: M' == M)) 
+    (exists M: multiset<nat> :: M in I && GSumNat(M) * 2 <= E && 
+                                I[M] == 1 &&
+                                forall M': multiset<nat> | M' in I && M' != M :: GSumNat(M') * 2 > E) 
 }
-
+/*
 lemma allMoreThanHalfFullImplies2Aproximated(A: multiset<nat>, E: nat, I: multiset<multiset<nat>>)
 requires isEnvasado(A, E, I)
 requires allMoreThanHalfFull(E, I) 
@@ -33,12 +36,181 @@ ensures isKAproximatedBinPacking(A, E, I, 2)
 {
     assume false;
 }
+*/
+
+//Used locally by atMostOneLessThanHalfImplies2Aproximated
+lemma multiplyingByNaturals(a: nat, b: nat, c: nat)
+requires a <= b
+ensures a * c <= b * c
+{ }
+
+//Used locally by dividingByNaturals
+lemma multiplyingByNaturals2(a: nat, b: nat, c: nat)
+requires a < b
+requires c > 0
+ensures a * c < b * c
+{ }
+
+//Used locally by atMostOneLessThanHalfImplies2Aproximated
+lemma dividingByNaturals(a: nat, b: nat, c: nat)
+requires a * c < b * c
+requires c > 0
+ensures a < b
+{
+    if a >= b {
+        multiplyingByNaturals(b, a, c);
+    }
+}
+
+//Used locally by atMostOneLessThanHalfImplies2Aproximated
+lemma commutativeProduct(a: nat, b: nat, c: nat)
+ensures a * b * c == a * c *b
+{ }
+
+//Used locally by atMostOneLessThanHalfImplies2Aproximated
+lemma distributivity(a: nat, b: nat, c: nat)
+ensures (a - b) * c + b * c == a * c 
+{ }
+
+//Used locally by atMostOneLessThanHalfImplies2Aproximated
+lemma productSimplification(a: nat, b: nat)
+ensures a * b + b == (a + 1) * b
+{ }
+
+//Used locally by atMostOneLessThanHalfImplies2Aproximated
+lemma lowerBoundSum(I: multiset<multiset<nat>>, E: nat, pesoTotal: nat)
+//y es E, z es pesoTotal
+requires forall i | i in I :: GSumNat(i) * 2 > E
+requires GMultisetSumNat(I) == pesoTotal
+ensures (I != multiset{} && |I| * E < pesoTotal * 2) || (I == multiset{} && pesoTotal * 2 == |I| * E)
+{
+    if I == multiset{} {}
+    else{
+        var i: multiset<nat> :| i in I;
+        var I' := I - multiset{i};
+        GMultisetSumNatIn(I, i);
+        lowerBoundSum(I', E, pesoTotal - GSumNat(i));
+
+        assert (pesoTotal - GSumNat(i)) * 2 >= |I'| * E;
+
+        assert GSumNat(i) * 2 > E;
+        assert (pesoTotal - GSumNat(i)) * 2 + GSumNat(i) * 2 > |I'| * E + E;
+        distributivity(pesoTotal, GSumNat(i), 2);
+        assert (pesoTotal - GSumNat(i)) * 2 + GSumNat(i) * 2 == pesoTotal * 2;
+
+        productSimplification(|I'|, E);
+        assert |I'| * E + E == (|I'| + 1) * E;
+        assert |I'| + 1 == |I|;
+        assert |I'| * E + E == |I| * E;
+
+        assert pesoTotal * 2 > |I| * E;
+    }
+}
+
+//Used locally by multisetsMoreThanHalf
+lemma isSmallerThan(a: nat, b: nat, c: nat)
+requires a == b - c 
+requires c > 0
+ensures a < b  
+{ }
+
+//Used locally by atMostOneLessThanHalfImplies2Aproximated
+ghost function multisetsMoreThanHalf(A: multiset<nat>, E: nat, I: multiset<multiset<nat>>): (I': multiset<multiset<nat>>)
+requires isEnvasado(A, E, I)
+requires forall i | i in I :: GSumNat(i) > 0
+requires allMoreThanHalfFull(E, I) || oneLessThanHalfFull(E, I)
+requires E > 0
+requires I != multiset{}
+ensures I' <= I 
+ensures |I'| + 1 == |I|
+ensures forall i' | i' in I' :: GSumNat(i') * 2 > E
+ensures GMultisetSumNat(I') < GSumNat(A)
+{
+    var pesoTotal := GSumNat(A);
+    if oneLessThanHalfFull(E, I) then
+        var lessThanHalf: multiset<nat> :| lessThanHalf in I && GSumNat(lessThanHalf) * 2 <= E;
+        var I' := I - multiset{lessThanHalf}; 
+        assert forall x | x in I' :: GSumNat(x) * 2 > E;
+        var diff := GSumNat(lessThanHalf);
+        GMultisetSumNatIn(I, lessThanHalf);
+        assert GMultisetSumNat(I) ==  GSumNat(lessThanHalf) + GMultisetSumNat(I - multiset{lessThanHalf});
+        GSumNatPartes2(A, I);
+        assert pesoTotal == diff + GMultisetSumNat(I');
+        var pesoTotal' := pesoTotal - diff;
+        assert diff > 0;
+        isSmallerThan(pesoTotal', pesoTotal, diff);
+        assert pesoTotal' == GMultisetSumNat(I');
+        I'
+    else 
+        var i :| i in I;
+        var I' := I - multiset{i};
+        var diff := GSumNat(i);
+        GMultisetSumNatIn(I, i);
+        assert GMultisetSumNat(I) ==  GSumNat(i) + GMultisetSumNat(I - multiset{i});
+        GSumNatPartes2(A, I);
+        assert pesoTotal == diff + GMultisetSumNat(I');
+        var pesoTotal' := pesoTotal - diff;
+        assert diff > 0;
+        assert pesoTotal' < pesoTotal;
+        I'
+}
+
+//Used locally by atMostOneLessThanHalfImplies2Aproximated
+lemma atMostOneLessThanHalfImplies2AproximatedCalc(A: multiset<nat>, E: nat, O: multiset<multiset<nat>>, I: multiset<multiset<nat>>, I': multiset<multiset<nat>>)
+requires isEnvasado(A, E, I)
+requires forall i | i in I :: GSumNat(i) > 0
+requires allMoreThanHalfFull(E, I) || oneLessThanHalfFull(E, I)
+requires E > 0
+requires I != multiset{}
+requires optimalEnvasado(A, E, O)
+requires I' == multisetsMoreThanHalf(A, E, I)
+ensures |I'| < |O| * 2
+{
+    var pesoTotal := GSumNat(A);
+    var pesoTotal' := GMultisetSumNat(I');
+
+    calc{
+        pesoTotal;
+        <= {lowerBoundoptimalValueEnvasado(A, E, O);}
+        |O| * E;
+    }
+    lowerBoundSum(I', E, pesoTotal');
+    assert |I'| * E <= pesoTotal' * 2;
+    calc{
+        |I'| * E;
+        <= 
+        pesoTotal' * 2;
+        < {multiplyingByNaturals(pesoTotal', pesoTotal, 2);}
+        pesoTotal * 2;
+        <= {multiplyingByNaturals(pesoTotal, |O| * E, 2);}
+        |O| * E * 2;
+        == {commutativeProduct(|O|, E, 2);}
+        |O| * 2 * E;
+    }
+    dividingByNaturals(|I'|, |O| * 2, E);
+    assert |I'| < |O| * 2;
+}
+
 
 lemma atMostOneLessThanHalfImplies2Aproximated(A: multiset<nat>, E: nat, I: multiset<multiset<nat>>)
 requires isEnvasado(A, E, I)
 requires allMoreThanHalfFull(E, I) || oneLessThanHalfFull(E, I) 
+requires E > 0
+requires forall i | i in I :: GSumNat(i) > 0
 ensures isKAproximatedBinPacking(A, E, I, 2)
 {
-    if allMoreThanHalfFull(E, I){allMoreThanHalfFullImplies2Aproximated(A, E, I);}
-    else{oneLessThanHalfFullImplies2Aproximated(A, E, I); }
+    if I == multiset{}{}
+    else{
+        var I' := multisetsMoreThanHalf(A, E, I);
+        enVasadoImpliesOptimalEnvasado(A, E, I);
+        var O: multiset<multiset<nat>> :| optimalEnvasado(A, E, O);
+
+        atMostOneLessThanHalfImplies2AproximatedCalc(A, E, O, I, I');
+        forall M: multiset<multiset<nat>> | isEnvasado(A, E, M)
+        ensures |I'| < |M| * 2
+        {
+            assert |O| <= |M|;
+            multiplyingByNaturals(|O|, |M|, 2);
+        }
+    }
 }
